some progress on the formalization

coq/Heapster.v
@@ -1,10 +1,22 @@
 Require Import ZArith List String Omega.
-Require Import ExtLib.Structures.Monads.
-Require Import ExtLib.Programming.Eqv.
+
+From Coq Require Import
+ Setoids.Setoid
+ Classes.Morphisms
+ Relations.Relations.
+
+From ExtLib Require Import
+     Structures.Monads
+     Programming.Eqv
+     Data.Monads.OptionMonad.
+
 Require Import FSets.FMapAVL.
 Require Coq.Structures.OrderedTypeEx.
 Require Import ZMicromega.
 Require Import Heapster.Int64.
+
+Import MonadNotation.
+Open Scope monad_scope.
 
 
 (* Maps from Z to values.  Used for contexts and environments *)
@@ -29,7 +41,7 @@ Inductive op :=
 
 Definition ctxt := ZMap arg.
 
-Definition lbl := Z.  (* Or i64? *)
+Definition lbl := i64.  (* Or i64? *)
 
 Inductive stmt :=
 | Load  (r:reg) (a:arg)   (*  r <- *a *)
@@ -38,7 +50,7 @@ Inductive stmt :=
 | Alloca (r:reg) (a:arg)
 | Malloc (r:reg) (a:arg)
 | Free   (a:arg)
-| Call   (l:lbl) (c:ctxt)
+| Call   (r:reg) (a:arg) (c:ctxt)
 .
 
 Definition tgt := (lbl * ctxt)%type.
@@ -109,11 +121,11 @@ Inductive allocate (H:heap) (bytes:i64) (l:tag) : val -> heap -> Prop :=
                    (Hp_aligned: aligned p 3 = true)
                    (Hbytes_mul8 : aligned bytes 3 = true)
                    (Hbytes_nz : Int64.ltu Int64.zero bytes = true)
-                   (HFree: forall i, in_range i p (Int64.add i bytes) = true ->
+                   (HFree: forall i, in_range i p (Int64.add p bytes) = true ->
                                 lookup i H = None)
-                   (HFresh: forall i, in_range i p (Int64.add i bytes) = true ->
+                   (HFresh: forall i, in_range i p (Int64.add p bytes) = true ->
                                  lookup i H' = Some (Uninit l p))
-                   (HSame: forall i, in_range i p (Int64.add i bytes) = false ->
+                   (HSame: forall i, in_range i p (Int64.add p bytes) = false ->
                                 lookup i H' = lookup i H),
     allocate H bytes l p H'.
 
@@ -127,6 +139,18 @@ Definition eval_arg_f (r:regs) (a:arg) : option val :=
 Inductive eval_arg (r:regs) (a:arg) : val -> Prop :=
 | eval_a : forall v (Heq: eval_arg_f r a = Some v), eval_arg r a v.
 
+
+Definition eval_binding (R:regs) (r:Z) (a:arg) (oR':option regs) : option regs := 
+  v <- eval_arg_f R a ;;
+  R' <- oR' ;;
+  ret (ZM.add r v R').
+
+Definition eval_ctxt_f (R:regs) (c:ctxt) : option regs :=
+  ZM.fold (eval_binding R) c (Some (@ZM.empty val)).
+
+Inductive eval_ctxt R c : regs -> Prop :=
+| eval_ctxt_a : forall R' (Heq: eval_ctxt_f R c = Some R'), eval_ctxt R c R'.
+
 Inductive eval_op : op -> val -> val -> val -> Prop :=
 | eval_add : forall (x y z : i64) (Heq: Int64.add x y = z), eval_op Add x y z
 | eval_sub : forall (x y z : i64) (Heq: Int64.sub x y = z), eval_op Sub x y z
@@ -135,25 +159,40 @@ Inductive eval_op : op -> val -> val -> val -> Prop :=
 | eval_ltt : forall (x y : i64) (Heq: Int64.lt x y = true), eval_op Lt x y Int64.one
 | eval_ltf : forall (x y : i64) (Heq: Int64.lt x y = false), eval_op Lt x y Int64.zero.
 
-Definition fresh_for_heapval (h:hv) (l:tag) : bool :=
+Definition used_in_heapval (h:hv) (l:tag) : bool := 
   match h with
-  | Code _ => true
-  | Uninit l' _ => negb (Z.eqb l l')
-  | Init l' _ _ => negb (Z.eqb l l')
+  | Code _ => false
+  | Uninit l' _ => Z.eqb l l'
+  | Init l' _ _ => Z.eqb l l'
   end.
 
-Definition fresh_for_heap (H:heap) (l:tag) : bool :=
-  IM.fold (fun _ h b => andb b (fresh_for_heapval h l)) H true.
+Definition fresh_for_heapval (h:hv) (l:tag) : bool :=
+  negb (used_in_heapval h l).
 
-Definition fresh_for_stack (s:stack) (l:tag) : Prop :=
-  not (In l (List.map (fun '(_, l', _, _) => l') s)).
+Definition used_in_heap (H:heap) (l:tag) : bool :=
+  IM.fold (fun _ h b => orb b (used_in_heapval h l)) H false.
+
+Definition fresh_for_heap (H:heap) (l:tag) : bool :=
+  negb (used_in_heap H l).
+
+Check List.fold_left.
+
+Definition lbls_in_stack (s:stack) : list tag :=
+  List.map (fun '(_, l', _, _) => l') s.
+
+Definition used_in_stack (s:stack) (l:tag) : bool :=
+  List.existsb (Z.eqb l) (lbls_in_stack s).
+
+Definition fresh_for_stack (s:stack) (l:tag) : bool :=
+  negb (used_in_stack s l).
+
+Definition used_in_config (c:config) (l:tag) : bool :=
+  let '(H, u, s, _, l', _) := c in
+  used_in_heap H l || used_in_stack s l || List.existsb (Z.eqb l) u || Z.eqb l l'.
 
 Definition fresh (c:config) (l:tag) : Prop :=
-  let '(H, u, s, _, l', _) := c in
-  fresh_for_heap H l = true /\
-  fresh_for_stack s l /\
-  not (In l u) /\
-  l <> l'.
+  used_in_config c l = false.
+
 
 (* SAZ: todo rewrite this using a filter, which would be more pleasant *)
 Definition free_heap (H:heap) (l:tag) : heap :=
@@ -208,13 +247,173 @@ Inductive step : config -> config -> Prop :=
     eval_arg R a1 x ->
     heap_root H x l' ->
     step (H, u, s, R, l, I (Free a1) cd)
-         (free_heap H l', l'::u, s, R, l, cd).
+         (free_heap H l', l'::u, s, R, l, cd)
+
+| step_call : forall H u s R R'  l l' cd cd' r a1 args x,
+    eval_arg R a1 x ->
+    lookup x H = Some (Code cd') ->
+    eval_ctxt R args R' ->
+    fresh (H, u, s, R, l, I (Call r a1 args) cd) l' ->
+    step (H, u, s, R, l, I (Call r a1 args) cd)
+         (H, u, (R, l, r, cd)::s, R', l', cd')
+
+| step_ret : forall H u s R R'  l l' cd' r' a1 x,
+    eval_arg R a1 x ->
+    step (H, u, (R', l', r', cd')::s, R, l, T (Ret a1))
+         (free_heap H l, l::u, s, ZM.add r' x R', l', cd')
+
+| step_jmp :  forall H u s R R'  l lbl cd' args,
+    lookup lbl H = Some (Code cd') ->
+    eval_ctxt R args R' ->
+    step (H, u, s, R, l, T (Jmp (lbl, args) ))
+         (H, u, s, R', l, cd')
+
+| step_brz0 : forall H u s R R'  l a1 lbl0 cd' args0 lbl_nz args_nz,
+    eval_arg R a1 Int64.zero ->
+    lookup lbl0 H = Some (Code cd') ->
+    eval_ctxt R args0 R' ->
+    step (H, u, s, R, l, T (Brz a1 (lbl0, args0) (lbl_nz, args_nz)))
+         (H, u, s, R', l, cd')
+
+| step_brz_nz : forall H u s R R'  l a1 x lbl0 cd' args0 lbl_nz args_nz,
+    eval_arg R a1 x ->
+    Int64.eq x Int64.zero = false ->
+    lookup lbl_nz H = Some (Code cd') ->
+    eval_ctxt R args_nz R' ->
+    step (H, u, s, R, l, T (Brz a1 (lbl0, args0) (lbl_nz, args_nz)))
+         (H, u, s, R', l, cd')
+
+.
+
+
+Lemma used_store_f_monotonic : forall H a v l H'
+                                 (Hused: used_in_heap H l = true)
+                                 (Hstore: store_f H a v = Some H'),
+    used_in_heap H' l = true.
+Proof.
+Admitted.
+
+Lemma used_allocate_monotonic1 : forall H a v l l0 H'
+                                 (Hused: used_in_heap H l = true)
+                                 (Hstore: allocate H a l0 v H'),
+    used_in_heap H' l = true.
+Proof.
+  intros H a v l l0 H' Hused Hstore.
+  inversion Hstore. subst.
+Admitted.
+
+Lemma used_allocate_monotonic2 : forall H a v l0 H'
+                                 (Hstore: allocate H a l0 v H'),
+    used_in_heap H' l0 = true.
+Proof.
+  intros H a v l0 H' Hstore.
+  inversion Hstore. subst.
+Admitted.
+
+
+
+Lemma used_monotonic : forall l c1 c2
+                         (Hused: (used_in_config c1 l = true) )
+                         (Hstep: step c1 c2),
+    used_in_config c2 l = true.
+Proof.
+  intros l c1 c2 Hused Hstep.
+  inversion Hstep; subst; simpl in *; try assumption.
+  - inversion H2.
+    subst.
+    destruct (used_in_heap H l) eqn:Hheap.
+    assert (used_in_heap H' l = true).
+    eapply used_store_f_monotonic; eauto. subst.
+    rewrite H3. assumption.
+    destruct (used_in_heap H' l) eqn:Hheap'.
+    reflexivity. assumption.
+Admitted.
+
+Inductive finished (x:i64) : config -> Prop :=
+| finished_c : forall H u R l a,
+    eval_arg R a x ->
+    finished x (H, u, nil, R, l, T (Ret a)).
+
+Definition stuck (c:config) :=
+ (~ exists x, finished x c) /\ ~ exists c', step c c'.
+
+Inductive streamF (A:Type) (X:Type) :=
+| snil : streamF A X
+| scons : A -> X -> streamF A X.
+
+
+CoInductive stream (A:Type) := go {
+  observe : streamF A (stream A)
+}.
+
+Set Implicit Arguments.
+
+Notation "#" := (go _ (snil _ _)).
+Notation "x >> s" := (go _ (scons _ _ x s)) (at level 100).
+
+
+Inductive runF (P : config -> stream config -> Prop) : config -> stream config -> Prop :=
+ | run_finished : forall c1 x, finished x c1 -> runF P c1 (c1 >> #)
+ | run_step : forall c1 c2 s, step c1 c2 -> P c2 s -> runF P c1 (c1 >> s)
+.
+
+CoInductive runC (c:config) (s:stream config) : Prop := goRun {
+  run_ : runF runC c s
+}.
+
+
+Lemma looping_config :
+  forall H lbl args u s R l,
+    lookup lbl H = Some (Code (T (Jmp (lbl, args)))) ->
+    eval_ctxt R args R ->
+    step (H, u, s, R, l, T (Jmp (lbl, args))) (H, u, s, R, l, T (Jmp (lbl, args))).
+Proof.
+  intros H lbl0 args u s R l H0 H1.
+  apply step_jmp; assumption.
+Qed.
+
+
+Section Permissions.
+
+  Record perm := mkPerm {
+    view : heap -> heap -> Prop;  (* PER over heaps *)
+    upd : heap -> heap -> Prop;   (* allowed transitions *)
+  }.
+
+  Record goodPerm (p:perm) : Prop := {
+     view_PER   : PER heap (view p) ;
+     upd_PO     : PreOrder (upd p) ;
+     upd_proper : Proper ((view p) ==> (view p) ==> iff) (upd p);
+  }.
+
+
+
+  Record lte_perm (p q:perm) : Prop := {
+     view_inc : forall x y, (view q) x y -> (view p) x y;
+     upd_inc : forall x y, (upd p) x y -> (upd q) x y;
+  }.
+
+  Record sep_at (p q:perm) (x:heap) : Prop := {
+    upd1: forall y:heap, (upd p) x y -> (view q) x y;
+    upd2: forall y:heap, (upd q) x y -> (view p) x y;
+  }.
+
+
+  Definition separate (p q : perm) : Prop := forall x, sep_at p q x.
+
+  Lemma separate_anti_monotone : forall (p1 p2 q : perm) (HSep: separate p2 q) (Hlt: lte_perm p1 p2),
+      separate p1 q.
+  Proof.
+    intros p1 p2 q HSep Hlt.
+    destruct Hlt.
+    unfold separate in HSep.
+    unfold separate.
+    intros. constructor; intuition.
+    apply HSep. intuition.
+    apply view_inc0. apply HSep. assumption.
+  Qed.
 
 
 
 
-
-
-
-
-
+End Permissions.
